src/lib/state/DY.Lib.State.PKI.fst
@@ -80,8 +80,8 @@ val has_pki_invariant: protocol_invariants -> prop
 let has_pki_invariant invs =
   has_map_session_invariant invs pki_pred
 
-val pki_tag_and_invariant: {|crypto_invariants|} -> string & session_pred
-let pki_tag_and_invariant #ci = (pki_types.tag, local_state_predicate_to_session_pred (map_session_invariant pki_pred))
+val pki_tag_and_invariant: {|crypto_invariants|} -> string & local_bytes_state_predicate
+let pki_tag_and_invariant #ci = (pki_types.tag, local_state_predicate_to_local_bytes_state_predicate (map_session_invariant pki_pred))
 
 (*** PKI API ***)
 
